\begin{document}

\section{Componential form of the equations of motions}\label{componential-form-of-the-equations-of-motion}
It turns convenient to derive the componential form of the equations of motion by differentiating the first equation with respect to s.
Notice that the second equations has only one component along $\mathbf{e}_3$.
We begin by writing the components of $\mathbf{T}_s$, $\mathbf{F}_{extart}$ and $\rho$S$\mathbf{r}_{tt}$ along $\mathbf{a}$ and $\mathbf{b}$. From $\mathbf{T}=N\mathbf{a}+H\mathbf{b}$ we get
\begin{equation}
\begin{split}
\mathbf{T}_{ss}& =((N\mathbf{a}+H\mathbf{b})_s)_s\\
               & =((N_s\mathbf{a}+ N\mathbf{a}_s + H_s\mathbf{b} + H\mathbf{b}_s)_s\\
               & = N_{ss}\mathbf{a} + N_s\mathbf{a}_s + N_s\mathbf{a}_s + N\mathbf{a}_{ss} + H_{ss}\mathbf{b} + H_s\mathbf{b}_s + H_s\mathbf{b}_s + H\mathbf{b}_{ss}.
\end{split}
\end{equation}
Exploiting the fact that $\mathbf{a}=(cos\theta, sen\theta)$ and $\mathbf{b}=(-sen\theta, cos\theta)$ we can express $\mathbf{a}_s$, $\mathbf{a}_{ss}, \mathbf{b}_s, \mathbf{b}_{ss}$ in terms of $\mathbf{a}$ and $\mathbf{b}$ only :

\begin{align}
\mathbf{a}   & = (cos\theta,sen\theta)                        &\mathbf{b}& = (-sen\theta, cos\theta)\\\\
\mathbf{a}_s & = ((-sen\theta)\theta_s, (cos\theta)\theta_s)  &\mathbf{b}_s& = ((-cos\theta)\theta_s, (-sen\theta)\theta_s)\\
             & = \theta_s(-sen\theta, cos\theta)              & &= \theta_s(-(cos\theta, sen\theta))\\
             & =\theta_s\mathbf{b}                            & &= -\theta_s\mathbf{a}\\\\
\mathbf{a}_{ss}& = \theta_{ss}\mathbf{b}+\theta_s\mathbf{b}_s & 
\mathbf{b}_{ss}& = -\theta_{ss}\mathbf{a}+\theta_s\mathbf{a}_s\\
               & = \theta_{ss}\mathbf{b} - \theta_s\theta_s\mathbf{a} & &= -\theta_{ss}\mathbf{a} -\theta_s\theta_s\mathbf{b}\\
               & = \theta_{ss}\mathbf{b} - \theta_s^2\mathbf{a} & &= -\theta_{ss}\mathbf{a} -\theta_s^2\mathbf{b}.
\end{align}

By substituting, we find that
\begin{equation}
\begin{split}
\mathbf{T}_{ss}& = N_{ss}\mathbf{a} + 2N_s(\theta_s\mathbf{b}) + N(\theta_{ss}\mathbf{b}-\theta_s^2\mathbf{a}) + H_{ss}\mathbf{b} + 2H_s(-\theta_s\mathbf{a}) + H(-\theta_{ss}\mathbf{a}-\theta_s^2\mathbf{b})\\
               & = N_{ss}\mathbf{a} + 2\theta_sN_s\mathbf{b}- N\theta_s^2\mathbf{a} + N\theta_ss\mathbf{b} + H_{ss}\mathbf{b} -2\theta_sH_s\mathbf{a}-H\theta_s^2\mathbf{b}-H\theta_{ss}\mathbf{a}\\
               & = (N_ss -2\theta_sH_s - H\theta_ss-N\theta_s^2)\mathbf{a} + (H_ss+2\theta_sN_s + N\theta_ss -H\theta_s^2)\mathbf{b}.
\end{split}
\end{equation}
Doing the same for $(\rho S\mathbf{r}_{tt})_s$ and exploiting the fact that 
\begin{align}
\mathbf{a}_t    &=\theta_t\mathbf{b} & \mathbf{b}_t &= -\theta_t\mathbf{a}\\
\mathbf{a}_{tt} &=\theta_{tt}\mathbf{b}-\theta_t^2\mathbf{a} & \mathbf{b}_{tt} &= -\theta_{tt}\mathbf{a}-\theta_t^2\mathbf{b} 
\end{align}
yields
\begin{equation}
\begin{split}
\rho S(\mathbf{r}_{tt})_s &= \rho S (\mathbf{r}_s)_{tt}\\
                          &= \rho S ((\nu\mathbf{a} + \eta\mathbf{b})_t)_t\\
                          &= \rho S (\nu_t\mathbf{a} + \nu\mathbf{a}_t + \eta_t\mathbf{b} + \eta\mathbf{b}_t)_t\\
                          &= \rho S (\nu_{tt}\mathbf{a} + \nu_t\mathbf{a}_t + \nu_t\mathbf{a}_t + \nu\mathbf{a}_{tt} + \eta_{tt}\mathbf{b} + \eta_t\mathbf{b}_t + \eta_t\mathbf{b}_t + \eta\mathbf{b}_{tt})\\
                          &= \rho S (\nu_{tt}\mathbf{a} + 2\nu_t\mathbf{a}_t + \nu\mathbf{a}_{tt} + \eta_{tt}\mathbf{b} + 2\eta_t\mathbf{b}_t + \eta\mathbf{b}_{tt})\\
                          &= \rho S (\nu_{tt}\mathbf{a} + 2\nu_t(\theta_t\mathbf{b}) + \nu(\theta_{tt}\mathbf{b}-\nu\theta_t^2\mathbf{a}) + \eta_{tt}\mathbf{b} + 2\eta_t(-\theta_t\mathbf{a}) + \eta(-\theta_{tt}\mathbf{a}-\theta_t^2\mathbf{b}))\\
                          &= \rho S (\nu_{tt}\mathbf{a} + 2\nu_t\theta_t\mathbf{b} + \nu\theta_{tt}\mathbf{b}-\nu\theta_t^2\mathbf{a}) + \eta_{tt}\mathbf{b} - 2\theta_t\eta_t\mathbf{a}) - \eta\theta_{tt}\mathbf{a} - \eta\theta_t^2\mathbf{b})\\
                          &= \rho S \left[ (\nu_{tt}-\nu\theta_t^2 - 2\theta_t\eta_t -\eta\theta_{tt})\mathbf{a} + (\nu\theta_{tt} + 2\theta_t\nu_t + \eta_{tt} - \eta\theta_t^2)\mathbf{b} \right]\\
                          &= \rho S (\nu_{tt} - 2\theta_t\eta_t -\eta\theta_{tt} - nu\theta_t^2  )\mathbf{a} + (\eta_{tt}+ 2\theta_t\nu_t + \nu\theta_{tt} - \eta\theta_t^2)\mathbf{b}).
\end{split}
\end{equation}




\end{document} 
  
  
  
  
  
  
  
  
  
  
  
  
  
  
  
  
  
  
  
  
  
  
  
  
  
  
  